cedar-lean/Cedar/TPE/BatchedEvaluator.lean
@@ -17,6 +17,7 @@
 
 import Cedar.Spec
 import Cedar.Data
+import Cedar.TPE.Authorizer
 import Cedar.TPE.Residual
 import Cedar.TPE.Evaluator
 import Cedar.TPE.Input
@@ -37,12 +38,12 @@ See `EntityLoader.WellBehaved` for a formal definition.
 abbrev EntityLoader := Set EntityUID → Map EntityUID MaybeEntityData
 
 /--
-The batched evaluation loop
+The batched evaluation loop for a single residual expression.
   1. Asks for any new entities referenced by the residual
   2. Partially evaluates now that new entities are loaded
   3. Exits if a value has been found or it hits the maximum iteration limit
 -/
-def batchedEvalLoop
+def batchedEvaluateLoop
   (residual : Residual)
   (req : Request)
   (loader : EntityLoader)
@@ -56,11 +57,10 @@ def batchedEvalLoop
 
     match Cedar.TPE.evaluate residual req.asPartialRequest newStore with
     | .val v _ty => .val v _ty
-    | newRes => batchedEvalLoop newRes req loader newStore n
-
+    | newRes => batchedEvaluateLoop newRes req loader newStore n
 
 /--
-Evaluate a cedar expression using an EntityLoader
+Evaluate a single cedar expression using an EntityLoader
 instead of a full Entities store.
 Performs a maximum of `iter` number of calls to `loader`,
 but may perform fewer when a value is found.
@@ -72,8 +72,45 @@ def batchedEvaluate
   (iters : Nat)
   : Residual :=
   let residual := Cedar.TPE.evaluate x.toResidual req.asPartialRequest Map.empty
-  -- start the batched evaluation loop
-  batchedEvalLoop residual req loader Map.empty iters
+  batchedEvaluateLoop residual req loader Map.empty iters
+
+/--
+The batched authorization loop for authorization over a list of policies.
+-/
+def batchedAuthorizeLoop
+  (residuals : List ResidualPolicy) (req : Request) (loader : EntityLoader)
+  (store : PartialEntities) (n : Nat)
+  : Response
+:=
+  let resp := isAuthorizedFromResiduals residuals
+  if resp.decision.isSome then
+    resp
+  else match n with
+    | 0 => resp
+    | n + 1 =>
+      let toLoad := residuals.mapUnion (λ rp : ResidualPolicy => rp.residual.allLiteralUIDs)|>.filter (λ uid => (store.find? uid).isNone)
+      let newEntities := ((loader toLoad).mapOnValues MaybeEntityData.asPartial)
+      let newStore := newEntities ++ store
+
+      let residuals : List ResidualPolicy := residuals.map λ rp =>
+        ⟨rp.id, rp.effect, Cedar.TPE.evaluate rp.residual req.asPartialRequest newStore⟩
+      batchedAuthorizeLoop residuals req loader newStore n
+
+/--
+Evaluate an authorization request using an EntityLoader instead of a full Entities store.
+
+Performs a maximum of `iter` number of calls to `loader`, but may perform fewer when an authorization decision is reached early.
+-/
+def batchedAuthorize
+  (schema : Schema)
+  (policies : List Policy)
+  (req : Request)
+  (loader : EntityLoader)
+  (iters : Nat)
+  : Except Error Response := do
+  let residualPolicies ← policies.mapM (λ p => do
+    pure ⟨p.id, p.effect, ← evaluatePolicy schema p req.asPartialRequest Map.empty⟩)
+  pure (batchedAuthorizeLoop residualPolicies req loader Map.empty iters)
 
 /--
 Create an entity loader for a given entity store.
