cedar-lean/Cedar/Thm/BatchedEvaluator/Evaluate.lean
@@ -1,0 +1,64 @@
+import Cedar.TPE.Input
+import Cedar.TPE.BatchedEvaluator
+import Cedar.Spec
+import Cedar.Validation
+import Cedar.Thm.Validation
+import Cedar.Thm.TPE
+import Cedar.Thm.BatchedEvaluator.Common
+
+/-!
+Soundness of batched expression evaluation: batched evaluation of a single
+well-typed residual produces the same result as direct evaluation with the
+complete entity store.
+-/
+
+namespace Cedar.Thm
+
+open Cedar.TPE
+open Cedar.Spec
+open Cedar.Validation
+open Cedar.Thm
+open Cedar.Data
+
+theorem batched_evaluate_loop_eq_evaluate
+  {x : Residual}
+  {req : Request}
+  (es : Entities)
+  {current_store : PartialEntities}
+  {env : TypeEnv} :
+  EntityLoader.WellBehaved es loader →
+  Residual.WellTyped env x →
+  RequestAndEntitiesRefine req es req.asPartialRequest current_store →
+  InstanceOfWellFormedEnvironment req es env →
+  (Residual.evaluate (batchedEvaluateLoop x req loader current_store iters) req es).toOption = (Residual.evaluate x req es).toOption := by
+  intro h₀ h₁ h₂ h₃
+  unfold batchedEvaluateLoop
+  split
+  case h_1 => simp only
+  case h_2 iters n=>
+    let toLoad := (Set.filter (fun uid => (Map.find? current_store uid).isNone) x.allLiteralUIDs)
+    let newEntities := ((loader toLoad).mapOnValues MaybeEntityData.asPartial)
+    let newStore := newEntities ++ current_store
+
+    have h₆ : RequestAndEntitiesRefine req es req.asPartialRequest newStore := by
+      constructor
+      · exact as_partial_request_refines
+      · apply entities_refine_append
+        · exact h₂.right
+        · exact (h₀ toLoad).2
+    let newRes := TPE.evaluate x req.asPartialRequest newStore
+    have h₇ : (Residual.evaluate newRes req es).toOption = (Residual.evaluate x req es).toOption := by
+      rw [← partial_evaluate_is_sound h₁ h₃ h₆]
+
+    simp only
+    split
+    case h_1 h₆ =>
+      rw [← h₆]
+      exact h₇
+    case h_2 =>
+      have h₈ := (partial_eval_preserves_well_typed h₃ h₆ h₁)
+      rw [batched_evaluate_loop_eq_evaluate es h₀ h₈ h₆ h₃]
+      exact h₇
+
+
+end Cedar.Thm
